Changed QHoare semantics.

thys/Registers/QHoare.thy
@@ -8,58 +8,67 @@ locale qhoare =
   fixes memory_type :: "'mem itself"
 begin
 
-type_synonym 'm statement = \<open>'m update list\<close>
-type_synonym 'm program = \<open>'m statement list\<close>
+type_synonym 'm statement = \<open>'m ell2 \<Rightarrow> 'm ell2 list\<close>
 
-definition \<open>seq P Q = [q o\<^sub>C\<^sub>L p. p \<leftarrow> P, q \<leftarrow> Q]\<close> for P Q :: \<open>'mem statement\<close>
-definition \<open>program S = foldr seq S [id_cblinfun]\<close> for S :: \<open>'mem program\<close>
-definition \<open>apply U R = [R U]\<close> for R :: \<open>'a update \<Rightarrow> 'mem update\<close>
-definition \<open>ifthenelse R M P Q = seq [R (Proj (ccspan (ket ` M)))] (program P) @
-                                 seq [R (Proj (ccspan (ket ` (-M))))] (program Q)\<close>
-  for R :: \<open>'a update \<Rightarrow> 'mem update\<close> and P Q :: \<open>'mem program\<close>
+definition \<open>seq P Q \<psi> = [\<gamma>. \<phi> \<leftarrow> P \<psi>, \<gamma> \<leftarrow> Q \<phi>]\<close> for P Q :: \<open>'mem statement\<close>
+definition skip :: \<open>'m statement\<close> where \<open>skip \<psi> = [\<psi>]\<close>
+definition \<open>program S = foldr seq S skip\<close> for S :: \<open>'mem statement list\<close>
+  \<comment> \<open>Convenience abbreviation: List of statements as repeated seq\<close>
+definition \<open>apply U R \<psi> = [R U *\<^sub>V \<psi>]\<close> for R :: \<open>'a update \<Rightarrow> 'mem update\<close>
+definition \<open>ifthenelse R M P Q \<psi> = P (R (Proj (ccspan (ket ` M))) \<psi>) @
+                                   Q (R (Proj (ccspan (ket ` (-M)))) \<psi>)\<close>
+  for R :: \<open>'a update \<Rightarrow> 'mem update\<close> and P Q :: \<open>'mem statement\<close>
 
-definition hoare :: \<open>'mem ell2 ccsubspace \<Rightarrow> 'mem program \<Rightarrow> 'mem ell2 ccsubspace \<Rightarrow> bool\<close> where
-  \<open>hoare C p D \<longleftrightarrow> (\<forall>\<psi> \<in> space_as_set C. \<forall>A \<in> set (program p). A *\<^sub>V \<psi> \<in> space_as_set D)\<close> for C p D
+definition hoare :: \<open>'mem ell2 ccsubspace \<Rightarrow> 'mem statement \<Rightarrow> 'mem ell2 ccsubspace \<Rightarrow> bool\<close> where
+  \<open>hoare C p D \<longleftrightarrow> (\<forall>\<psi> \<in> space_as_set C. set (p \<psi>) \<subseteq> space_as_set D)\<close> for C p D
 
 definition EQ :: \<open>('a update \<Rightarrow> 'mem update) \<Rightarrow> 'a ell2 \<Rightarrow> 'mem ell2 ccsubspace\<close> (infix "=\<^sub>q" 75) where
   \<open>EQ R \<psi> = R (proj \<psi>) *\<^sub>S \<top>\<close>
 
+lemma seq_skip[simp]: \<open>seq P skip = P\<close> and \<open>seq skip P = P\<close>
+  by (auto simp: seq_def skip_def)
+
 lemma seq_assoc: \<open>seq (seq P Q) R = seq P (seq Q R)\<close>
-  apply (induction P)
-  by (simp_all add: map_concat o_def seq_def cblinfun_compose_assoc)
+proof (rule ext)
+  fix \<psi>
+  define P\<psi> where \<open>P\<psi> = P \<psi>\<close>
+  show \<open>seq (seq P Q) R \<psi> = seq P (seq Q R) \<psi>\<close>
+    apply (simp add: seq_def flip: P\<psi>_def)
+    apply (induction P\<psi>)
+    by auto
+qed
 
 lemma program_seq: \<open>program (p1@p2) = seq (program p1) (program p2)\<close>
   apply (induction p1)
-   apply (simp add: program_def seq_def)
+   apply (simp add: program_def seq_def skip_def)
   by (simp add: program_def seq_assoc)
 
-lemma hoare_seq[trans]: \<open>hoare C p1 D \<Longrightarrow> hoare D p2 E \<Longrightarrow> hoare C (p1@p2) E\<close>
-  by (auto simp: program_seq hoare_def seq_def)
+lemma hoare_seq[trans]: \<open>hoare C p1 D \<Longrightarrow> hoare D p2 E \<Longrightarrow> hoare C (seq p1 p2) E\<close>
+  by (auto simp: hoare_def seq_def)
 
 lemma hoare_weaken_left[trans]: \<open>A \<le> B \<Longrightarrow> hoare B p C \<Longrightarrow> hoare A p C\<close>
   unfolding hoare_def
   by (meson in_mono less_eq_ccsubspace.rep_eq) 
 
 lemma hoare_weaken_right[trans]: \<open>hoare A p B \<Longrightarrow> B \<le> C \<Longrightarrow> hoare A p C\<close>
-  unfolding hoare_def 
-  by (meson in_mono less_eq_ccsubspace.rep_eq) 
+  by (auto simp add: hoare_def less_eq_ccsubspace.rep_eq)
 
-lemma hoare_skip: \<open>C \<le> D \<Longrightarrow> hoare C [] D\<close>
-  by (auto simp: program_def hoare_def in_mono less_eq_ccsubspace.rep_eq)
+lemma hoare_skip: \<open>C \<le> D \<Longrightarrow> hoare C skip D\<close>
+  by (auto simp: skip_def hoare_def less_eq_ccsubspace.rep_eq)
 
 lemma hoare_apply: 
   assumes \<open>R U *\<^sub>S pre \<le> post\<close>
-  shows \<open>hoare pre [apply U R] post\<close>
-  using assms apply (auto simp: hoare_def program_def apply_def seq_def)
+  shows \<open>hoare pre (apply U R) post\<close>
+  using assms apply (auto simp: hoare_def apply_def seq_def)
   by (metis (no_types, lifting) cblinfun_image.rep_eq closure_subset imageI less_eq_ccsubspace.rep_eq subsetD)
 
 lemma hoare_ifthenelse:
   fixes R :: \<open>'a update \<Rightarrow> 'mem update\<close>
   assumes \<open>hoare (R (Proj (ccspan (ket ` M))) *\<^sub>S pre) P post\<close>
   assumes \<open>hoare (R (Proj (ccspan (ket ` (-M)))) *\<^sub>S pre) Q post\<close>
-  shows \<open>hoare pre [ifthenelse R M P Q] post\<close>
+  shows \<open>hoare pre (ifthenelse R M P Q) post\<close>
   using assms
-  by (auto simp: program_def[of \<open>[_]\<close>] hoare_def ifthenelse_def butterfly_def seq_def cblinfun_apply_in_image')
+  by (auto simp: hoare_def ifthenelse_def cblinfun_apply_in_image')
 
 end
 
